theories/Dot/dot_syn.v
@@ -3,6 +3,9 @@ From D Require Export prelude tactics asubst_base.
 
 Definition label := string.
 
+Module sort_instances.
+Import autosubst_instances.
+
 Inductive tm : Type :=
   | tv : vl_ -> tm
   | tapp : tm -> tm -> tm
@@ -481,7 +484,10 @@ Instance hsubst_lemmas_dms : HSubstLemmas vl dms := _.
 
 Include Sorts.
 
-Instance sort_tm: Sort tm := {}.
-Instance sort_dm: Sort dm := {}.
-Instance sort_path: Sort path := {}.
-Instance sort_ty: Sort ty := {}.
+Global Instance sort_tm: Sort tm := {}.
+Global Instance sort_dm: Sort dm := {}.
+Global Instance sort_path: Sort path := {}.
+Global Instance sort_ty: Sort ty := {}.
+End sort_instances.
+
+Export sort_instances.
